Typing.v
@@ -2,9 +2,9 @@ From stdpp Require Import mapset.
 From CT Require Import CoreLangProp.
 From CT Require Import OperationalSemantics.
 From CT Require Import BasicTypingProp.
-From CT Require Import RefinementType.
+From CT Require Import TransducerProp.
+From CT Require Import RefinementTypeProp.
 From CT Require Import Denotation.
-From CT Require Import Instantiation.
 From CT Require Import InstantiationProp.
 
 Import Atom.
@@ -15,90 +15,85 @@ Import ListCtx.
 Import Trace.
 Import OperationalSemantics.
 Import BasicTyping.
+Import Qualifier.
+Import Transducer.
 Import RefinementType.
 Import Denotation.
 Import Instantiation.
-Import Qualifier.
+
 
 (** This file formalizes the type system of λᴱ and the main metatheoretic
   results. *)
 
 (** Well-formedness (Fig. 5) *)
-Definition wf_am (Γ: listctx pty) (A: am): Prop := closed_am (ctxdom Γ) A.
+(* Definition wf_td (Γ: listctx rty) (A: transducer): Prop := closed_td (ctxdom Γ) A. *)
 
-Definition prefix_am (Γ: listctx pty) (A B: am) : Prop :=
-  forall Γv, ctxRst Γ Γv ->
-        forall α, a⟦m{ Γv }a B⟧ α →
-             a⟦m{ Γv }a A ;+ ∘*⟧ α.
+(* Definition prefix_td (Γ: listctx rty) (A B: transducer) : Prop := *)
+(*   forall Γv, ctxRst Γ Γv -> *)
+(*         forall α, a⟦m{ Γv }a B⟧ α → *)
+(*              a⟦m{ Γv }a A ;+ ∘*⟧ α. *)
 
-Inductive wf_pty: listctx pty -> pty -> Prop :=
-| WfBase: forall Γ b ϕ,
-    closed_pty (ctxdom Γ) {: b | ϕ } -> wf_pty Γ {: b | ϕ }
-| WfArr: forall Γ ρ τ (L: aset),
-    wf_pty Γ ρ ->
-    (forall x, x ∉ L -> wf_hty (Γ ++ [(x, ρ)]) (τ ^h^ x)) ->
-    wf_pty Γ (ρ ⇨ τ)
-| WfGhost: forall Γ b ρ (L: aset),
-    (forall x, x ∉ L -> wf_pty (Γ ++ [(x, mk_top b)]) (ρ ^p^ x)) ->
-    wf_pty Γ (b ⇢ ρ)
+(* Definition wf_rty (Γ: listctx rty) (τ: rty): Prop := closed_rty (ctxdom Γ) τ. *)
+(* | WfOver: forall Γ b ϕ, *)
+(*     closed_rty (ctxdom Γ) {: b | ϕ } -> wf_rty Γ {: b | ϕ } *)
+(* | WfUnder: forall Γ b ϕ a, *)
+(*     closed_rty (ctxdom Γ) [: b | ϕ ]!<[ a ]> -> *)
+(*     wf_td *)
+(*     wf_rty Γ [: b | ϕ ]!<[ a ]> *)
+(* | WfArr: forall Γ ρ τ (L: aset), *)
+(*     wf_rty Γ ρ -> *)
+(*     (forall x, x ∉ L -> wf_rty (Γ ++ [(x, ρ)]) (τ ^h^ x)) -> *)
+(*     wf_rty Γ (ρ ⇨ τ) *)
+(* | WfGhost: forall Γ b ρ (L: aset), *)
+(*     (forall x, x ∉ L -> wf_rty (Γ ++ [(x, mk_top b)]) (ρ ^p^ x)) -> *)
+(*     wf_rty Γ (b ⇢ ρ) *)
 
-with wf_hty: listctx pty -> hty -> Prop :=
-| WfHoare: forall Γ ρ A B,
-    wf_pty Γ ρ ->
-    wf_am Γ A ->
-    wf_am Γ B ->
-    prefix_am Γ A B ->
-    wf_hty Γ (<[ A ] ρ [ B ]>)
-| WfInter: forall Γ τ1 τ2,
-    wf_hty Γ τ1 ->
-    wf_hty Γ τ2 ->
-    ⌊ τ1 ⌋ = ⌊ τ2 ⌋ ->
-    wf_hty Γ (τ1 ⊓ τ2)
-.
+(* with wf_rty: listctx rty -> rty -> Prop := *)
+(* | WfHoare: forall Γ ρ A B, *)
+(*     wf_rty Γ ρ -> *)
+(*     wf_td Γ A -> *)
+(*     wf_td Γ B -> *)
+(*     prefix_td Γ A B -> *)
+(*     wf_rty Γ (<[ A ] ρ [ B ]>) *)
+(* | WfInter: forall Γ τ1 τ2, *)
+(*     wf_rty Γ τ1 -> *)
+(*     wf_rty Γ τ2 -> *)
+(*     ⌊ τ1 ⌋ = ⌊ τ2 ⌋ -> *)
+(*     wf_rty Γ (τ1 ⊓ τ2) *)
+(* . *)
 
-Notation " Γ '⊢WF' τ " := (wf_hty Γ τ) (at level 20, τ constr, Γ constr).
-Notation " Γ '⊢WFp' τ " := (wf_pty Γ τ) (at level 20, τ constr, Γ constr).
-Notation " Γ '⊢WFa' a " := (wf_am Γ a) (at level 20, a constr, Γ constr).
+Notation " Γ '⊢WF' τ " := (closed_rty (ctxdom Γ) τ) (at level 20, τ constr, Γ constr).
+Notation " Γ '⊢WFa' a " := (closed_td (ctxdom Γ) a) (at level 20, a constr, Γ constr).
 
-Reserved Notation "Γ '⊢' e '⋮t' τ" (at level 20).
-Reserved Notation "Γ '⊢' e '⋮v' τ"  (at level 20).
+Reserved Notation "Γ '⊢' e '⋮' τ"  (at level 20).
 
 (** Semantic subtyping *)
 (* Instead of the syntactic subtyping relation presented in the paper, we use
 semantic subtyping in the mechanization. *)
-Definition pty_subtyping (Γ: listctx pty) (ρ1 ρ2: pty) : Prop :=
-  (* Assume [ρ1] and [ρ2] are valid [pty]s. *)
+Definition subtyping (Γ: listctx rty) (ρ1 ρ2: rty) : Prop :=
+  (* Assume [ρ1] and [ρ2] are valid [rty]s. *)
   ⌊ ρ1 ⌋ = ⌊ ρ2 ⌋ /\
   forall Γv, ctxRst Γ Γv ->
-        forall e, p⟦m{ Γv }p ρ1⟧ e →
-             p⟦m{ Γv }p ρ2⟧ e.
+        forall e, ⟦m{ Γv }r ρ1⟧ e → ⟦m{ Γv }r ρ2⟧ e.
 
-Definition subtyping (Γ: listctx pty) (τ1 τ2: hty) : Prop :=
-  (* Assume [τ1] and [τ2] are valid [hty]s. *)
-  ⌊ τ1 ⌋ = ⌊ τ2 ⌋ /\
-  forall Γv, ctxRst Γ Γv ->
-        forall e, ⟦m{ Γv }h τ1⟧ e →
-             ⟦m{ Γv }h τ2⟧ e.
-
-Notation " Γ '⊢' ρ1 '<⋮p' ρ2 " := (pty_subtyping Γ ρ1 ρ2) (at level 20, ρ1 constr, ρ2 constr, Γ constr).
 Notation " Γ '⊢' τ1 '<⋮' τ2 " := (subtyping Γ τ1 τ2) (at level 20, τ1 constr, τ2 constr, Γ constr).
 
 (* The builtin typing relation (Δ) that our type system is parameterized over. *)
-Parameter builtin_typing_relation : effop -> pty -> Prop.
+Parameter builtin_typing_relation : effop -> rty -> Prop.
 
 Reserved Notation "Γ '⊢' op '⋮o' ρ"  (at level 20).
 Reserved Notation "Γ '⊢' e '⋮t' τ" (at level 20).
-Reserved Notation "Γ '⊢' e '⋮v' ρ"  (at level 20).
+Reserved Notation "Γ '⊢' e '⋮v' τ" (at level 20).
 
 (** * Typing rules (Fig. 6) *)
 
-Inductive effop_type_check : listctx pty -> effop -> pty -> Prop :=
+Inductive effop_type_check : listctx rty -> effop -> rty -> Prop :=
 | TEOp : forall Γ op ρ_op ρ,
-    Γ ⊢WFp ρ ->
+    Γ ⊢WF ρ ->
     builtin_typing_relation op ρ_op ->
     (* [TSubEOp] is inlined here. Consecutive applications of subtyping is just
     one subtyping. *)
-    Γ ⊢ ρ_op <⋮p ρ ->
+    Γ ⊢ ρ_op <⋮ ρ ->
     ⌊ ρ ⌋ = ty_of_op op ->
     Γ ⊢ op ⋮o ρ
 where
@@ -106,87 +101,90 @@ where
 
 (** Typing rules for values and terms. Values always have refinement types, while
   terms always have Hoare automata types. *)
-Inductive term_type_check : listctx pty -> tm -> hty -> Prop :=
-| TEPur: forall Γ v ρ A,
-    Γ ⊢WF (<[ A ] ρ [ A ]>) ->
+Inductive term_type_check : listctx rty -> tm -> rty -> Prop :=
+| TEPur: forall Γ v ρ,
+    Γ ⊢WF (ρ !<[ tdId ]>) ->
     Γ ⊢ v ⋮v ρ ->
-    Γ ⊢ v ⋮t (<[ A ] ρ [ A ]>)
-| TSub: forall Γ e (τ1 τ2: hty),
+    Γ ⊢ v ⋮t (ρ !<[ tdId ]>)
+| TSub: forall Γ e (τ1 τ2: rty),
     Γ ⊢WF τ2 ->
     Γ ⊢ e ⋮t τ1 ->
     Γ ⊢ τ1 <⋮ τ2 ->
     Γ ⊢ e ⋮t τ2
-| TInter: forall Γ e (τ1 τ2: hty),
-    Γ ⊢WF (τ1 ⊓ τ2) ->
-    Γ ⊢ e ⋮t τ1 ->
-    Γ ⊢ e ⋮t τ2 ->
-    Γ ⊢ e ⋮t (τ1 ⊓ τ2)
-| TLetE: forall Γ e_x e ρx ρ A A' B (L: aset),
-    Γ ⊢WF (<[ A ] ρ [ B ]>) ->
-    Γ ⊢ e_x ⋮t (<[ A ] ρx [ A' ]>) ->
+| TLetEBase: forall Γ e1 e2 b1 ϕ1 A1 τ2 A2 (L: aset),
     (forall x, x ∉ L ->
-          (Γ ++ [(x, ρx)]) ⊢ (e ^t^ x) ⋮t (<[ A' ] ρ [ B ]>)) ->
-    Γ ⊢ (tlete e_x e) ⋮t (<[ A ] ρ [ B ]>)
-| TApp: forall Γ (v1 v2: value) e ρ ρx ρ2 A A' B (L: aset),
-    Γ ⊢WF (<[ (A ^a^ v2) ] ρ [ B ]>) ->
+          (Γ ++ [(x, {: b1 | ϕ1})]) ⊢ (e2 ^t^ x) ⋮t (τ2 !<[ A2 ]>)) ->
+    Γ ⊢WF (τ2!<[ (tdEx b1 ϕ1 A1) ○ A2 ]>) ->
+    Γ ⊢ e1 ⋮t ([: b1 | ϕ1]!<[ A1 ]>) ->
+    Γ ⊢ (tlete e1 e2) ⋮t (τ2!<[ (tdEx b1 ϕ1 A1) ○ A2 ]>)
+| TLetEArr: forall Γ e1 e2 ρ1 τ1 A1 τ2 A2 (L: aset),
+    (forall x, x ∉ L ->
+          (Γ ++ [(x, ρ1 ⇨ τ1)]) ⊢ (e2 ^t^ x) ⋮t (τ2 !<[ A2 ]>)) ->
+    Γ ⊢WF (τ2!<[ A1 ○ A2 ]>) ->
+    Γ ⊢ e1 ⋮t (ρ1 ⇨ τ1 !<[ A1 ]>) ->
+    Γ ⊢ (tlete e1 e2) ⋮t (τ2!<[ A1 ○ A2 ]>)
+| TAppBase: forall Γ (v1 v2: value) e ρ2 b1 ϕ1 A1 τ2 A2 (L: aset),
+    (forall x, x ∉ L ->
+          (Γ ++ [(x, {: b1 | ϕ1} ^r^ v2)]) ⊢ (e ^t^ x) ⋮t (τ2 !<[ A2 ]>)) ->
+    Γ ⊢WF (τ2!<[ ((tdEx b1 ϕ1 A1) ^a^ v2) ○ A2 ]>) ->
     Γ ⊢ v2 ⋮v ρ2 ->
-    Γ ⊢ v1 ⋮v (ρ2 ⇨ (<[ A ] ρx [ A' ]>)) ->
+    Γ ⊢ v1 ⋮v (ρ2 ⇨ ([: b1 | ϕ1]!<[A1]>)) ->
+    Γ ⊢ (tletapp v1 v2 e) ⋮t (τ2!<[ ((tdEx b1 ϕ1 A1) ^a^ v2) ○ A2 ]>)
+| TAppArr: forall Γ (v1 v2: value) e ρ2 ρ11 ρ12 A1 τ2 A2 (L: aset),
     (forall x, x ∉ L ->
-          (Γ ++ [(x, ρx ^p^ v2)]) ⊢ (e ^t^ x) ⋮t (<[ A' ^a^ v2 ] ρ [ B ]>)) ->
-    Γ ⊢ (tletapp v1 v2 e) ⋮t (<[ A ^a^ v2 ] ρ [ B ]>)
-| TEOpApp: forall Γ (op: effop) (v2: value) e ρ ρx ρ2 A A' B (L: aset),
-    Γ ⊢WF (<[ A ^a^ v2 ] ρ [ B ]>) ->
+          (Γ ++ [(x, (ρ11 ⇨ ρ12) ^r^ v2)]) ⊢ (e ^t^ x) ⋮t (τ2 !<[ A2 ]>)) ->
+    Γ ⊢WF (τ2!<[ (A1 ^a^ v2) ○ A2 ]>) ->
     Γ ⊢ v2 ⋮v ρ2 ->
-    Γ ⊢ op ⋮o (ρ2 ⇨ (<[ A ] ρx [ A' ]>)) ->
+    Γ ⊢ v1 ⋮v (ρ2 ⇨ (ρ11 ⇨ ρ12!<[A1]>)) ->
+    Γ ⊢ (tletapp v1 v2 e) ⋮t (τ2!<[ (A1 ^a^ v2) ○ A2 ]>)
+| TAppOp: forall Γ (op: effop) (v2: value) e ρ2 b1 ϕ1 A1 τ2 A2 (L: aset),
     (forall x, x ∉ L ->
-          (Γ ++ [(x, ρx ^p^ v2)]) ⊢ (e ^t^ x) ⋮t (<[ A' ^a^ v2 ] ρ [ B ]>)) ->
-    Γ ⊢ (tleteffop op v2 e) ⋮t (<[ A ^a^ v2 ] ρ [ B ]>)
+          (Γ ++ [(x, {: b1 | ϕ1} ^r^ v2)]) ⊢ (e ^t^ x) ⋮t (τ2 !<[ A2 ]>)) ->
+    Γ ⊢WF (τ2!<[ (A1 ^a^ v2) ○ A2 ]>) ->
+    Γ ⊢ v2 ⋮v ρ2 ->
+    Γ ⊢ op ⋮o (ρ2 ⇨ ([: b1 | ϕ1]!<[A1]>)) ->
+    Γ ⊢ (tleteffop op v2 e) ⋮t (τ2!<[ (A1 ^a^ v2) ○ A2 ]>)
 | TMatchb: forall Γ (v: value) e1 e2 ϕ τ (L : aset),
     Γ ⊢WF τ ->
     Γ ⊢ v ⋮v {:TBool | ϕ} ->
-    (* We can also directly encode the path condition without mentioning [x]:
-    {: TNat | (qual [# v] (fun V => V !!! 0 = (cbool true))%fin) & ϕ ^q^ v} *)
+    (* We can also directly encode the path condition without mentioning [x]: *)
+(*     {: TNat | (qual [# v] (fun V => V !!! 0 = (cbool true))%fin) & ϕ ^q^ v} *)
     (forall x, x ∉ L -> (Γ ++ [(x, {: TBool | b0:c=true & b0:v= v & ϕ})]) ⊢ e1 ⋮t τ) ->
     (forall x, x ∉ L -> (Γ ++ [(x, {: TBool | b0:c=false & b0:v= v & ϕ})]) ⊢ e2 ⋮t τ) ->
     Γ ⊢ (tmatchb v e1 e2) ⋮t τ
-with value_type_check : listctx pty -> value -> pty -> Prop :=
-| TSubPP: forall Γ (v: value) (ρ1 ρ2: pty),
-    Γ ⊢WFp ρ2 ->
+with value_type_check : listctx rty -> value -> rty -> Prop :=
+| TSubPP: forall Γ (v: value) (ρ1 ρ2: rty),
+    Γ ⊢WF ρ2 ->
     Γ ⊢ v ⋮v ρ1 ->
-    Γ ⊢ ρ1 <⋮p ρ2 ->
+    Γ ⊢ ρ1 <⋮ ρ2 ->
     Γ ⊢ v ⋮v ρ2
-| TGhost: forall Γ v b ρ (L: aset),
-    Γ ⊢WFp (b ⇢ ρ) ->
-    (forall (x: atom), x ∉ L -> (Γ ++ [(x, mk_top b)]) ⊢ v ⋮v (ρ ^p^ x)) ->
-    Γ ⊢ v ⋮v (b ⇢ ρ)
 | TConst: forall Γ (c: constant),
-    Γ ⊢WFp (mk_eq_constant c) ->
+    Γ ⊢WF (mk_eq_constant c) ->
     Γ ⊢ c ⋮v (mk_eq_constant c)
 | TBaseVar: forall Γ (x: atom) b ϕ,
-    Γ ⊢WFp (mk_eq_var b x) ->
+    Γ ⊢WF (mk_eq_var b x) ->
     ctxfind Γ x = Some {: b | ϕ} ->
     Γ ⊢ x ⋮v (mk_eq_var b x)
 | TFuncVar: forall Γ (x: atom) ρ τ,
-    Γ ⊢WFp (ρ ⇨ τ) ->
+    Γ ⊢WF (ρ ⇨ τ) ->
     ctxfind Γ x = Some (ρ ⇨ τ) ->
     Γ ⊢ x ⋮v (ρ ⇨ τ)
 | TFun: forall Γ Tx ρ e τ (L: aset),
-    Γ ⊢WFp (ρ ⇨ τ) ->
-    (forall x, x ∉ L -> (Γ ++ [(x, ρ)]) ⊢ (e ^t^ x) ⋮t (τ ^h^ x)) ->
+    Γ ⊢WF (ρ ⇨ τ) ->
+    (forall x, x ∉ L -> (Γ ++ [(x, ρ)]) ⊢ (e ^t^ x) ⋮t (τ ^r^ x)) ->
     Tx = ⌊ ρ ⌋ ->
     Γ ⊢ (vlam Tx e) ⋮v (ρ ⇨ τ)
 | TFix: forall Γ (Tx : base_ty) ϕ e τ T (L: aset),
-    Γ ⊢WFp ({: Tx | ϕ} ⇨ τ) ->
-    (* NOTE: should not open the whole type, because the first argument (bound
-    variable 0) of the return type is not the fixed point function but [{: Tx |
-    ϕ}]. The return type should be opened by [x]. *)
+    Γ ⊢WF ({: Tx | ϕ} ⇨ τ) ->
+    (* NOTE: should not open the whole type, because the first argument (bound *)
+(*     variable 0) of the return type is not the fixed point function but [{: Tx | *)
+(*     ϕ}]. The return type should be opened by [x]. *)
     (forall x, x ∉ L ->
-          (Γ ++ [(x, {: Tx | ϕ})]) ⊢ (vlam (Tx ⤍ T) e) ^v^ x ⋮v (({: Tx | b0:x≺ x & ϕ} ⇨ τ) ⇨ (τ ^h^ x))) ->
+          (Γ ++ [(x, {: Tx | ϕ})]) ⊢ (vlam (Tx ⤍ T) e) ^v^ x ⋮v (({: Tx | b0:x≺ x & ϕ} ⇨ τ) ⇨ (τ ^r^ x))) ->
     T = ⌊ τ ⌋ ->
     Γ ⊢ (vfix (Tx ⤍ T) (vlam (Tx ⤍ T) e)) ⋮v ({: Tx | ϕ} ⇨ τ)
 where
 "Γ '⊢' e '⋮t' τ" := (term_type_check Γ e τ) and "Γ '⊢' e '⋮v' ρ" := (value_type_check Γ e ρ).
-
 
 Scheme value_term_type_check_ind := Minimality for value_type_check Sort Prop
     with term_value_type_check_ind := Minimality for term_type_check Sort Prop.
@@ -202,8 +200,8 @@ Proof.
   qauto.
 Qed.
 
-Lemma pty_subtyping_preserves_basic_typing Γ ρ1 ρ2 :
-  Γ ⊢ ρ1 <⋮p ρ2 ->
+Lemma rty_subtyping_preserves_basic_typing Γ ρ1 ρ2 :
+  Γ ⊢ ρ1 <⋮ ρ2 ->
   ⌊ρ1⌋ = ⌊ρ2⌋.
 Proof.
   qauto.
@@ -216,58 +214,61 @@ Proof.
   inversion 1; subst. eauto.
 Qed.
 
-Lemma value_typing_regular_wf : forall (Γ: listctx pty) (v: value) (ρ: pty),
-    Γ ⊢ v ⋮v ρ -> wf_pty Γ ρ
-with tm_typing_regular_wf : forall (Γ: listctx pty) (e: tm) (τ: hty),
-    Γ ⊢ e ⋮t τ -> wf_hty Γ τ.
+Lemma value_typing_regular_wf : forall (Γ: listctx rty) (v: value) (ρ: rty),
+    Γ ⊢ v ⋮v ρ -> Γ ⊢WF ρ
+with tm_typing_regular_wf : forall (Γ: listctx rty) (e: tm) (τ: rty),
+    Γ ⊢ e ⋮t τ -> Γ ⊢WF τ.
 Proof.
   all: destruct 1; eauto.
 Qed.
 
 Lemma value_tm_typing_regular_basic_typing:
-  (forall (Γ: listctx pty) (v: value) (ρ: pty),
+  (forall (Γ: listctx rty) (v: value) (ρ: rty),
     Γ ⊢ v ⋮v ρ -> ⌊ Γ ⌋* ⊢t v ⋮v ⌊ ρ ⌋) /\
-  (forall (Γ: listctx pty) (e: tm) (τ: hty),
+  (forall (Γ: listctx rty) (e: tm) (τ: rty),
     Γ ⊢ e ⋮t τ -> ⌊ Γ ⌋* ⊢t e ⋮t ⌊ τ ⌋).
 Proof.
   apply value_term_type_check_mutind; intros; cbn; subst; eauto.
-  - hauto using pty_subtyping_preserves_basic_typing.
-  - auto_pose_fv x. repeat specialize_with x.
-    rewrite ctx_erase_app_r in H1 by my_set_solver.
-    rewrite <- pty_erase_open_eq in H1.
-    eapply basic_typing_strengthen_value; eauto. my_set_solver.
-  - econstructor.
-    qauto using ctx_erase_lookup.
-  - econstructor.
-    qauto using ctx_erase_lookup.
-  - econstructor.
+  - hauto using rty_subtyping_preserves_basic_typing.
+  - (* TBaseVar *) econstructor. qauto using ctx_erase_lookup.
+  - (* TFuncVar *) econstructor. qauto using ctx_erase_lookup.
+  - (* TFun *) econstructor.
     instantiate_atom_listctx.
     rewrite ctx_erase_app_r in H1 by my_set_solver.
-    rewrite <- hty_erase_open_eq in H1.
+    rewrite <- rty_erase_open_eq in H1.
     eauto.
-  - econstructor.
+  - (* TFix *) econstructor.
     instantiate_atom_listctx.
     rewrite ctx_erase_app_r in H1 by my_set_solver.
     cbn in H1.
-    rewrite <- hty_erase_open_eq in H1.
+    rewrite <- rty_erase_open_eq in H1.
     eauto.
   - hauto using subtyping_preserves_basic_typing.
   - econstructor; eauto.
     instantiate_atom_listctx.
-    rewrite ctx_erase_app_r in H3 by my_set_solver.
+    rewrite ctx_erase_app_r in H0 by my_set_solver.
+    eauto.
+  - econstructor; eauto.
+    instantiate_atom_listctx.
+    rewrite ctx_erase_app_r in H0 by my_set_solver.
     eauto.
   - econstructor.
-    cbn in H3. eauto. eauto.
+    cbn in H0. eauto. eauto.
     instantiate_atom_listctx.
-    rewrite ctx_erase_app_r in H5 by my_set_solver.
-    rewrite <- pty_erase_open_eq in H5.
+    rewrite ctx_erase_app_r in H0 by my_set_solver.
+    rewrite <- rty_erase_open_eq in H0.
     eauto.
-  - apply effop_typing_preserves_basic_typing in H2. cbn in H2. sinvert H2.
+  - econstructor.
+    cbn in H0. eauto. eauto.
+    instantiate_atom_listctx.
+    rewrite ctx_erase_app_r in H0 by my_set_solver.
+    rewrite <- rty_erase_open_eq in H0.
+    eauto.
+  - apply effop_typing_preserves_basic_typing in H4. cbn in H4. sinvert H4.
     econstructor; eauto. qauto.
     instantiate_atom_listctx.
-    rewrite ctx_erase_app_r in H4 by my_set_solver.
-    rewrite <- pty_erase_open_eq in H4.
-    rewrite <- H7. eauto.
+    rewrite ctx_erase_app_r in H0 by my_set_solver.
+    rewrite <- rty_erase_open_eq in H0; eauto.
   - auto_pose_fv x. repeat specialize_with x.
     rewrite ctx_erase_app_r in H3, H5 by my_set_solver.
     econstructor; eauto.
@@ -275,13 +276,13 @@ Proof.
     eapply basic_typing_strengthen_tm; eauto. my_set_solver.
 Qed.
 
-Lemma value_typing_regular_basic_typing: forall (Γ: listctx pty) (v: value) (ρ: pty),
+Lemma value_typing_regular_basic_typing: forall (Γ: listctx rty) (v: value) (ρ: rty),
     Γ ⊢ v ⋮v ρ -> ⌊ Γ ⌋* ⊢t v ⋮v ⌊ ρ ⌋.
 Proof.
   apply value_tm_typing_regular_basic_typing.
 Qed.
 
-Lemma tm_typing_regular_basic_typing: forall (Γ: listctx pty) (e: tm) (τ: hty),
+Lemma tm_typing_regular_basic_typing: forall (Γ: listctx rty) (e: tm) (τ: rty),
     Γ ⊢ e ⋮t τ -> ⌊ Γ ⌋* ⊢t e ⋮t ⌊ τ ⌋.
 Proof.
   apply value_tm_typing_regular_basic_typing.
@@ -290,18 +291,19 @@ Qed.
 Lemma ctxRst_insert_easy Γ env (x: atom) ρ (v: value):
     ctxRst Γ env ->
     x ∉ ctxdom Γ ->
-    p⟦ m{ env }p ρ ⟧ v ->
+    ⟦ m{ env }r ρ ⟧ v ->
+    pure_rty ρ ->
     ctxRst (Γ ++ [(x, ρ)]) (<[ x := v ]> env).
 Proof.
   intros. econstructor; eauto.
   econstructor; eauto using ctxRst_ok_ctx.
-  apply ptyR_typed_closed in H1. simp_hyps.
-  (* This should be a lemma similar to [msubst_preserves_closed_pty_empty], or
+  apply rtyR_typed_closed in H1. simp_hyps.
+  (* This should be a lemma similar to [msubst_preserves_closed_rty_empty], or
   we should strenghthen this lemma. But don't bother now as it is only used
   here. *)
-  sinvert H2.
-  econstructor. eauto using lc_msubst_pty, ctxRst_lc.
-  rewrite fv_of_msubst_pty_closed in H4 by eauto using ctxRst_closed_env.
+  sinvert H3.
+  econstructor. eauto using lc_msubst_rty, ctxRst_lc.
+  rewrite fv_of_msubst_rty_closed in H5 by eauto using ctxRst_closed_env.
   rewrite ctxRst_dom in * by eauto.
   my_set_solver.
 Qed.
@@ -309,7 +311,8 @@ Qed.
 Lemma ctxRst_ctxfind Γ Γv x ρ :
   ctxRst Γ Γv ->
   ctxfind Γ x = Some ρ ->
-  exists (v : value), Γv !! x = Some v /\ p⟦ m{ Γv }p ρ ⟧ v.
+  fine_rty ρ ->
+  exists (v : value), Γv !! x = Some v /\ ⟦ m{ Γv }r ρ ⟧ v.
 Proof.
   induction 1.
   - easy.
@@ -317,11 +320,11 @@ Proof.
     select (ctxfind (_ ++ _) _ = _)
       (fun H => apply ctxfind_app in H; eauto using ok_ctx_ok).
 
-    assert (forall (v' : value), (p⟦(m{env}p) ρ⟧) v' ->
-                            (p⟦(m{<[x0:=v]> env}p) ρ⟧) v'). {
-      select (p⟦ _ ⟧ _) (fun H => apply ptyR_typed_closed in H). simp_hyps.
+    assert (forall (v' : value), (⟦(m{env}r) ρ⟧) v' ->
+                            (⟦(m{<[x0:=v]> env}r) ρ⟧) v'). {
+      select (⟦ _ ⟧ _) (fun H => apply rtyR_typed_closed in H). simp_hyps.
       intros.
-      apply ptyR_msubst_insert_eq; eauto using ctxRst_closed_env.
+      apply rtyR_msubst_insert_eq; eauto using ctxRst_closed_env.
       select (_ ⊢t _ ⋮t _)
         (fun H => apply basic_typing_contains_fv_tm in H; simpl in H).
       my_set_solver.
@@ -330,7 +333,6 @@ Proof.
       simp_hyps.
       apply not_elem_of_dom. eauto.
     }
-
     destruct_or!; simp_hyps.
     + eexists. split; eauto.
       assert (x <> x0). {
@@ -344,627 +346,118 @@ Proof.
       eexists. split; eauto. by simplify_map_eq.
 Qed.
 
-Lemma wf_pty_closed Γ ρ :
-  wf_pty Γ ρ ->
-  closed_pty (ctxdom Γ) ρ
-with wf_hty_closed Γ τ :
-  wf_hty Γ τ ->
-  closed_hty (ctxdom Γ) τ.
-Proof.
-  all: destruct 1; eauto; split;
-    let go :=
-      repeat select (_ ⊢WFp _) (fun H => apply wf_pty_closed in H; sinvert H);
-      repeat select (_ ⊢WF _) (fun H => apply wf_hty_closed in H; sinvert H);
-      repeat destruct select (_ ⊢WFa _);
-      eauto in
-    match goal with
-    | |- lc_pty _ =>
-        repeat econstructor; try instantiate_atom_listctx; go
-    | |- lc_hty _ =>
-        repeat econstructor; try instantiate_atom_listctx; go
-    | |- _ =>
-        simpl; auto_pose_fv x; repeat specialize_with x; go;
-        rewrite <- ?open_fv_hty' in *;
-        rewrite <- ?open_fv_pty' in *;
-        rewrite ?ctxdom_app_union in *;
-        my_set_solver
-    end.
-Qed.
+(* Lemma wf_rty_closed Γ ρ : *)
+(*   Γ ⊢WF ρ -> closed_rty (ctxdom Γ) ρ. *)
+(* Proof. *)
+(*   all: destruct 1; eauto; split; *)
+(*     let go := *)
+(*       repeat select (_ ⊢WF _) (fun H => apply wf_rty_closed in H; sinvert H); *)
+(*       repeat destruct select (_ ⊢WFa _); *)
+(*       eauto in *)
+(*     match goal with *)
+(*     | |- lc_rty _ => *)
+(*         repeat econstructor; try instantiate_atom_listctx; go *)
+(*     | |- _ => *)
+(*         simpl; auto_pose_fv x; repeat specialize_with x; go; *)
+(*         rewrite <- ?open_fv_rty' in *; *)
+(*         rewrite <- ?open_fv_rty' in *; *)
+(*         rewrite ?ctxdom_app_union in *; *)
+(*         my_set_solver *)
+(*     end. *)
+(* Qed. *)
 
 Lemma denotation_application_lam Tx T ρ τ e :
   Tx ⤍ T = ⌊ ρ⇨τ ⌋ ->
   ∅ ⊢t vlam Tx e ⋮t Tx ⤍ T ->
-  closed_pty ∅ (ρ⇨τ) ->
+  closed_rty ∅ (ρ⇨τ) ->
   (forall (v_x : value),
-      p⟦ρ⟧ v_x ->
-      ⟦τ ^h^ v_x⟧ (e ^t^ v_x)) ->
-  (p⟦ρ⇨τ⟧) (vlam Tx e).
+      ⟦ρ⟧ v_x ->
+      ⟦τ ^r^ v_x⟧ (e ^t^ v_x)) ->
+  (⟦ρ⇨τ⟧) (vlam Tx e).
 Proof.
   intros He Ht Hc H.
   split; [| split]; eauto. sinvert He; eauto.
-  intros v_x HDv_x.
-  repeat rewrite_measure_irrelevant.
-  specialize (H v_x HDv_x).
-  eapply htyR_refine; cycle 1. eauto.
 
-  apply ptyR_typed_closed in HDv_x. simp_hyps. sinvert H0.
-  split; intros.
-  - apply htyR_typed_closed in H. destruct H as [H _].
-    repeat esplit. eauto.
-    rewrite <- hty_erase_open_eq.
-    sinvert He.
-    eapply mk_app_e_v_has_type; eauto.
-  - eapply reduction_letapplam; eauto using basic_typing_regular_value.
-Qed.
+Admitted.
+(*   intros v_x HDv_x. *)
+(*   repeat rewrite_measure_irrelevant. *)
+(*   specialize (H v_x HDv_x). *)
+(*   eapply rtyR_refine; cycle 1. eauto. *)
+
+(*   apply rtyR_typed_closed in HDv_x. simp_hyps. sinvert H0. *)
+(*   split; intros. *)
+(*   - apply rtyR_typed_closed in H. destruct H as [H _]. *)
+(*     repeat esplit. eauto. *)
+(*     rewrite <- rty_erase_open_eq. *)
+(*     sinvert He. *)
+(*     eapply mk_app_e_v_has_type; eauto. *)
+(*   - eapply reduction_letapplam; eauto using basic_typing_regular_value. *)
+(* Qed. *)
 
 Lemma denotation_application_fixed (Tx : base_ty) T ϕ τ e :
   T = ⌊ τ ⌋ ->
   ∅ ⊢t vfix (Tx ⤍ T) (vlam (Tx ⤍ T) e) ⋮v Tx ⤍ T ->
-  closed_pty ∅ ({:Tx|ϕ}⇨τ) ->
+  closed_rty ∅ ({:Tx|ϕ}⇨τ) ->
   (forall (v_x : value),
-      p⟦{:Tx | ϕ}⟧ v_x ->
-      p⟦({:Tx | (b0:v≺ v_x) & ϕ} ⇨ τ) ⇨ (τ ^h^ v_x)⟧
+      ⟦{:Tx | ϕ}⟧ v_x ->
+      ⟦({:Tx | (b0:v≺ v_x) & ϕ} ⇨ τ) ⇨ (τ ^r^ v_x)⟧
         ((vlam (Tx ⤍ T) e) ^v^ v_x)) ->
-  p⟦{:Tx | ϕ}⇨τ⟧ (vfix (Tx ⤍ T) (vlam (Tx ⤍ T) e)).
+  ⟦{:Tx | ϕ}⇨τ⟧ (vfix (Tx ⤍ T) (vlam (Tx ⤍ T) e)).
 Proof.
   intros He Ht Hc Hlam.
   split; [| split]; eauto. subst; eauto.
-  intros v_x HDc.
-  repeat rewrite_measure_irrelevant.
-  assert (exists c, v_x = vconst c) as H. {
-    apply ptyR_typed_closed in HDc.
-    destruct HDc as [H _]. sinvert H.
-    eauto using basic_typing_base_canonical_form.
-  }
-  destruct H as [c ->].
-  induction c using (well_founded_induction constant_lt_well_founded).
-  specialize (Hlam c HDc).
-  destruct Hlam as (HTlam&HClam&HDlam).
-  specialize (HDlam (vfix (Tx ⤍ T) (vlam (Tx ⤍ T) e))).
-  repeat rewrite_measure_irrelevant.
-  rewrite open_hty_idemp in HDlam by eauto using lc.
-  eapply htyR_refine; cycle 1.
-  apply HDlam.
-  split; [| split].
-  simpl. cbn. unfold erase, hty_erase_ in He. rewrite <- He. eauto.
-  sinvert HClam. econstructor. sinvert H0. eauto. my_set_solver.
-  intros v_y HDv_y.
-  repeat rewrite_measure_irrelevant.
-  assert (exists y, v_y = vconst y). {
-    apply ptyR_typed_closed in HDv_y.
-    destruct HDv_y as [HTv_y _]. sinvert HTv_y.
-    eauto using basic_typing_base_canonical_form.
-  }
-  destruct H0 as (y&->).
-  destruct HDv_y as (HTy&_&Hy).
-  ospecialize* (Hy _ []); eauto. destruct Hy as [_ Hy].
-  rewrite qualifier_and_open in Hy.
-  rewrite denote_qualifier_and in Hy.
-  simp_hyps.
-  apply H; eauto.
-  (* lemma? *)
-  apply ptyR_typed_closed in HDc. simp_hyps.
-  split; [| split]; eauto.
-  intros. apply value_reduction_refl in H4. simp_hyps.
-  intuition.
+Admitted.
+(*   intros v_x HDc. *)
+(*   repeat rewrite_measure_irrelevant. *)
+(*   assert (exists c, v_x = vconst c) as H. { *)
+(*     apply rtyR_typed_closed in HDc. *)
+(*     destruct HDc as [H _]. sinvert H. *)
+(*     eauto using basic_typing_base_canonical_form. *)
+(*   } *)
+(*   destruct H as [c ->]. *)
+(*   induction c using (well_founded_induction constant_lt_well_founded). *)
+(*   specialize (Hlam c HDc). *)
+(*   destruct Hlam as (HTlam&HClam&HDlam). *)
+(*   specialize (HDlam (vfix (Tx ⤍ T) (vlam (Tx ⤍ T) e))). *)
+(*   repeat rewrite_measure_irrelevant. *)
+(*   rewrite open_rty_idemp in HDlam by eauto using lc. *)
+(*   eapply rtyR_refine; cycle 1. *)
+(*   apply HDlam. *)
+(*   split; [| split]. *)
+(*   simpl. cbn. unfold erase, rty_erase_ in He. rewrite <- He. eauto. *)
+(*   sinvert HClam. econstructor. sinvert H0. eauto. my_set_solver. *)
+(*   intros v_y HDv_y. *)
+(*   repeat rewrite_measure_irrelevant. *)
+(*   assert (exists y, v_y = vconst y). { *)
+(*     apply rtyR_typed_closed in HDv_y. *)
+(*     destruct HDv_y as [HTv_y _]. sinvert HTv_y. *)
+(*     eauto using basic_typing_base_canonical_form. *)
+(*   } *)
+(*   destruct H0 as (y&->). *)
+(*   destruct HDv_y as (HTy&_&Hy). *)
+(*   ospecialize* (Hy _ []); eauto. destruct Hy as [_ Hy]. *)
+(*   rewrite qualifier_and_open in Hy. *)
+(*   rewrite denote_qualifier_and in Hy. *)
+(*   simp_hyps. *)
+(*   apply H; eauto. *)
+(*   (* lemma? *) *)
+(*   apply rtyR_typed_closed in HDc. simp_hyps. *)
+(*   split; [| split]; eauto. *)
+(*   intros. apply value_reduction_refl in H4. simp_hyps. *)
+(*   intuition. *)
 
-  split; intros.
-  - subst. cbn in HTlam.
-    repeat esplit.
-    eapply mk_app_e_v_has_type; eauto.
-    rewrite <- hty_erase_open_eq.
-    eapply mk_app_e_v_has_type; eauto.
-    apply ptyR_typed_closed in HDc. destruct HDc as [HTc _].
-    sinvert HTc. eauto.
-  - apply reduction_mk_app_e_v in H0.
-    sinvert H0. sinvert H1. simplify_list_eq.
-    apply reduction_mk_app_e_v' in H2.
-    eauto.
-    eauto using basic_typing_regular_value.
-Qed.
+(*   split; intros. *)
+(*   - subst. cbn in HTlam. *)
+(*     repeat esplit. *)
+(*     eapply mk_app_e_v_has_type; eauto. *)
+(*     rewrite <- rty_erase_open_eq. *)
+(*     eapply mk_app_e_v_has_type; eauto. *)
+(*     apply rtyR_typed_closed in HDc. destruct HDc as [HTc _]. *)
+(*     sinvert HTc. eauto. *)
+(*   - apply reduction_mk_app_e_v in H0. *)
+(*     sinvert H0. sinvert H1. simplify_list_eq. *)
+(*     apply reduction_mk_app_e_v' in H2. *)
+(*     eauto. *)
+(*     eauto using basic_typing_regular_value. *)
+(* Qed. *)
 
-
-(** * Main metatheoretic results *)
-
-(** Convert an event operator to a value:
-  [op] is [fun x => leteffop y = op x in y] *)
-Definition value_of_op op : value :=
-  vlam TNat (tleteffop op (vbvar 0) (vbvar 0)).
-
-(** Well-formed built-in operator typing context (Definition 4.7) *)
-(* We simply treat the event operator as a value. This is equivalent to the
-definition in the paper (if we expand the denotation of this value). *)
-Definition well_formed_builtin_typing :=
-  forall op ρ,
-    builtin_typing_relation op ρ ->
-    p⟦ ρ ⟧ (value_of_op op).
-
-Lemma msubst_value_of_op Γv op :
-  m{Γv}v (value_of_op op) = value_of_op op.
-Proof.
-  rewrite msubst_fresh_value. eauto.
-  my_set_solver.
-Qed.
-
-Lemma value_of_op_regular_basic_typing op:
-  ∅ ⊢t value_of_op op ⋮v ty_of_op op.
-Proof.
-  econstructor.
-  simpl. instantiate (1:=∅). intros.
-  econstructor. econstructor. simplify_map_eq. reflexivity. reflexivity.
-  instantiate_atom_listctx.
-  simpl. econstructor. econstructor. simplify_map_eq. reflexivity.
-Qed.
-
-(* At some point the proof is very slow without marking [msubst] opaque. *)
-Opaque msubst.
-
-Ltac simpl_fv :=
-  do_hyps (fun H => try match type of H with
-                    | _ ∉ _ =>
-                        simpl in H; rewrite ?ctxRst_dom in H by eassumption
-                    end).
-
-(** Fundamental theorem for event operator typing *)
-Lemma builtin_fundamental:
-  well_formed_builtin_typing ->
-  forall (Γ: listctx pty) (op: effop) (ρ : pty),
-    Γ ⊢ op ⋮o ρ ->
-    forall Γv, ctxRst Γ Γv -> p⟦ m{ Γv }p ρ ⟧ (value_of_op op).
-Proof.
-  intros HWF Γ op ρ Hop Γv HΓv. sinvert Hop.
-  apply H1; eauto.
-  apply HWF in H0.
-  rewrite msubst_fresh_pty; eauto.
-  apply ptyR_typed_closed in H0. simp_hyps.
-  sinvert H3.
-  my_set_solver.
-Qed.
-
-(** Combined fundamental theorem for value typing (refinemnet types) and term
-  typing (Hoare automata types) *)
-Theorem fundamental_combined:
-  well_formed_builtin_typing ->
-  (forall (Γ: listctx pty) (v: value) (ρ: pty),
-    Γ ⊢ v ⋮v ρ ->
-    forall Γv, ctxRst Γ Γv -> p⟦ m{Γv}p ρ ⟧ (m{Γv}v v)) /\
-  (forall (Γ: listctx pty) (e: tm) (τ: hty),
-    Γ ⊢ e ⋮t τ ->
-    forall Γv, ctxRst Γ Γv -> ⟦ m{ Γv }h τ ⟧ (m{ Γv }t e)).
-Proof.
-  intros HWFbuiltin.
-  apply value_term_type_check_mutind.
-  (* [TSubPP] *)
-  - intros Γ v ρ1 ρ2 HWFρ2 _ HDρ1 Hsub Γv HΓv. specialize (HDρ1 _ HΓv).
-    apply Hsub in HDρ1; auto.
-  (* [TGhost] *)
-  - intros Γ v b ρ L HWF Hv HDv Γv HΓv. repeat msubst_simp.
-    split; [| split]. {
-      assert (Γ ⊢ v ⋮v (b⇢ρ)) by eauto using value_type_check.
-      eapply value_typing_regular_basic_typing in H.
-      eapply msubst_preserves_basic_typing_value_empty in H; eauto.
-      econstructor. apply_eq H. cbn. apply pty_erase_msubst_eq.
-    } {
-      eapply_eq msubst_preserves_closed_pty_empty; eauto using wf_pty_closed.
-      msubst_simp.
-    }
-    auto_pose_fv x. repeat specialize_with x.
-    intros.
-    assert (ctxRst (Γ ++ [(x, mk_top b)]) (<[x:=v0]> Γv)) as HΓv'. {
-      eapply ctxRst_insert_easy; eauto. my_set_solver.
-      repeat msubst_simp. eauto using mk_top_denote_pty.
-    }
-    ospecialize* HDv; eauto.
-    rewrite <- msubst_intro_pty in HDv by
-      (eauto using ctxRst_closed_env, ctxRst_lc, basic_typing_closed_value;
-       simpl_fv; my_set_solver).
-    apply_eq HDv. by rewrite <- open_preserves_pty_measure.
-    rewrite msubst_insert_fresh_value by
-      (eauto using ctxRst_closed_env, basic_typing_closed_value;
-       simpl_fv; my_set_solver).
-    auto.
-  (* [TConst] *)
-  - intros Γ c HWF Γv HΓv. repeat msubst_simp. eauto using mk_eq_constant_denote_pty.
-  (* [TBaseVar] *)
-  - intros Γ x b ϕ Hwf Hfind Γv HΓv.
-    dup_hyp HΓv (fun H => eapply ctxRst_ctxfind in H; eauto). simp_hyps.
-    repeat msubst_simp. rewrite H0.
-    destruct H1 as [H _].
-    sinvert H. cbn in H3.
-    dup_hyp H3 (fun H => apply basic_typing_base_canonical_form in H).
-    simp_hyps. subst. sinvert H3.
-    eauto using mk_eq_constant_denote_pty.
-  (* [TFuncVar] *)
-  - intros Γ x ρ τ Hwf Hfind Γv HΓv.
-    dup_hyp HΓv (fun H => eapply ctxRst_ctxfind in H; eauto). simp_hyps.
-    repeat msubst_simp.
-    by rewrite H0.
-  (* [TFun] *)
-  - intros Γ Tx ρ e τ L HWF Ht HDe He Γv HΓv. repeat msubst_simp.
-    eapply denotation_application_lam; eauto.
-    cbn. rewrite <- pty_erase_msubst_eq, <- hty_erase_msubst_eq. subst. eauto.
-    {
-      assert (Γ ⊢ vlam Tx e ⋮v (ρ⇨τ)) by eauto using value_type_check.
-      eapply value_typing_regular_basic_typing in H.
-      eapply msubst_preserves_basic_typing_value_empty in H; eauto.
-      repeat msubst_simp.
-      econstructor. apply_eq H. cbn. subst. reflexivity.
-    } {
-      eapply_eq msubst_preserves_closed_pty_empty; eauto using wf_pty_closed.
-      msubst_simp.
-    }
-    intros v_x Hv_x.
-    auto_pose_fv x. repeat specialize_with x.
-    assert (ctxRst (Γ ++ [(x, ρ)]) (<[x:=v_x]> Γv)) as HΓv'. {
-      apply ctxRst_insert_easy; eauto. my_set_solver.
-    }
-    ospecialize* HDe; eauto.
-    rewrite <- msubst_intro_tm in HDe by
-        (eauto using ctxRst_closed_env, ctxRst_lc, ptyR_closed_value;
-         simpl_fv; my_set_solver).
-    rewrite <- msubst_intro_hty in HDe by
-        (eauto using ctxRst_closed_env, ctxRst_lc, ptyR_closed_value;
-         simpl_fv; my_set_solver).
-    eauto.
-  (* [TFix] *)
-  - intros Γ Tx ϕ e τ T L HWF Hlam HDlam He Γv HΓv. repeat msubst_simp.
-    eapply denotation_application_fixed; eauto.
-    by rewrite <- hty_erase_msubst_eq.
-    {
-      assert (Γ ⊢ vfix (Tx ⤍ T) (vlam (Tx ⤍ T) e) ⋮v ({:Tx|ϕ}⇨τ))
-        by eauto using value_type_check.
-      eapply value_typing_regular_basic_typing in H.
-      eapply msubst_preserves_basic_typing_value_empty in H; eauto.
-      repeat msubst_simp.
-      apply_eq H. cbn. subst. eauto.
-    } {
-      eapply_eq msubst_preserves_closed_pty_empty; eauto using wf_pty_closed.
-      repeat msubst_simp.
-    }
-    intros v_x Hv_x.
-    auto_pose_fv x. repeat specialize_with x.
-    assert (ctxRst (Γ ++ [(x, {:Tx|ϕ})]) (<[x:=v_x]> Γv)) as HΓv'. {
-      apply ctxRst_insert_easy; eauto. my_set_solver.
-      msubst_simp.
-    }
-    ospecialize* HDlam; eauto.
-    rewrite <- msubst_intro_value in HDlam by
-        (eauto using ctxRst_closed_env, ctxRst_lc, ptyR_closed_value;
-         simpl_fv; my_set_solver).
-    repeat msubst_simp.
-    rewrite <- msubst_intro_hty in HDlam by
-        (eauto using ctxRst_closed_env, ctxRst_lc, ptyR_closed_value;
-         simpl_fv; my_set_solver).
-    rewrite msubst_insert_fresh_hty in HDlam by
-      (eauto using ctxRst_closed_env, ptyR_closed_value; simpl_fv; my_set_solver).
-    rewrite_msubst msubst_qualifier in HDlam.
-    rewrite msubst_insert_fresh_qualifier in HDlam by
-      (eauto using ctxRst_closed_env, ptyR_closed_value; simpl_fv; my_set_solver).
-    apply_eq HDlam.
-    simpl. repeat msubst_simp.
-    clear. simplify_map_eq. eauto.
-  (* [TEPur] *)
-  - intros Γ v ρ A HWF Hv HDv Γv HΓv. specialize (HDv _ HΓv).
-    repeat msubst_simp.
-    split; [| split]. {
-      eapply value_typing_regular_basic_typing in Hv.
-      eapply msubst_preserves_basic_typing_value_empty in Hv; eauto.
-      cbn. rewrite <- pty_erase_msubst_eq. eauto.
-    } {
-      eapply_eq msubst_preserves_closed_hty_empty; eauto using wf_hty_closed.
-      repeat msubst_simp.
-    }
-    intros. rewrite_measure_irrelevant.
-    apply value_reduction_refl in H0. simp_hyps. subst. simpl_list. eauto.
-  (* [TSub] *)
-  - intros Γ e τ1 τ2 HWFτ2 _ HDτ1 Hsub Γv HΓv. specialize (HDτ1 _ HΓv).
-    apply Hsub in HDτ1; auto.
-  (* [TInter] *)
-  - intros Γ e τ1 τ2 HWF HT1 HD1 HT2 HD2 Γv HΓv. repeat msubst_simp.
-    split; [| split]. {
-      eapply tm_typing_regular_basic_typing in HT1.
-      eapply msubst_preserves_basic_typing_tm_empty in HT1; eauto.
-      cbn. rewrite <- hty_erase_msubst_eq. eauto.
-    } {
-      eapply_eq msubst_preserves_closed_hty_empty; eauto using wf_hty_closed.
-      repeat msubst_simp.
-    }
-    repeat rewrite_measure_irrelevant. eauto.
-  (* [TLetE] *)
-  - intros Γ e_x e ρx ρ A A' B L HWF HTe_x HDe_x HTe HDe Γv HΓv.
-    ospecialize* HDe_x; eauto. repeat msubst_simp.
-    split; [| split]. {
-      assert (Γ ⊢ tlete e_x e ⋮t (<[ A ] ρ [ B ]>)) by eauto using term_type_check.
-      eapply tm_typing_regular_basic_typing in H.
-      eapply msubst_preserves_basic_typing_tm_empty in H; eauto.
-      repeat msubst_simp.
-      apply_eq H. cbn. eauto using pty_erase_msubst_eq.
-    } {
-      eapply_eq msubst_preserves_closed_hty_empty; eauto using wf_hty_closed.
-      repeat msubst_simp.
-    }
-    intros α β v HDα Hstepv.
-    apply reduction_tlete in Hstepv.
-    destruct Hstepv as (βx & βe & v_x & -> & Hstepv_x & Hstepv).
-    auto_pose_fv x. repeat specialize_with x.
-    destruct HDe_x as (_ & _ & HDe_x).
-    ospecialize* HDe_x; eauto. destruct HDe_x as [HDv_x HDα_βx].
-    assert (ctxRst (Γ ++ [(x, ρx)]) (<[x:=v_x]> Γv)) as HΓv'. {
-      apply ctxRst_insert_easy; eauto. my_set_solver.
-    }
-    ospecialize* HDe; eauto.
-    rewrite <- msubst_intro_tm in HDe by
-        (eauto using ctxRst_closed_env, ctxRst_lc, ptyR_closed_value;
-         simpl_fv; my_set_solver).
-    repeat msubst_simp.
-    destruct HDe as (_ & _ & HDe).
-    rewrite msubst_insert_fresh_am in HDe by
-      (eauto using ctxRst_closed_env, ptyR_closed_value;
-       simpl_fv; my_set_solver).
-    ospecialize* HDe; eauto.
-    repeat rewrite_measure_irrelevant.
-    rewrite msubst_insert_fresh_pty in HDe by
-      (eauto using ctxRst_closed_env, ptyR_closed_value;
-       simpl_fv; my_set_solver).
-    rewrite msubst_insert_fresh_am in HDe by
-      (eauto using ctxRst_closed_env, ptyR_closed_value;
-       simpl_fv; my_set_solver).
-    clear - HDe.
-    by simplify_list_eq.
-  (* [TApp] *)
-  - intros Γ v1 v2 e ρ ρx ρ2 A A' B L HWF HTv2 HDv2 HTv1 HDv1 HTe HDe Γv HΓv.
-    ospecialize* HDv1; eauto. ospecialize* HDv2; eauto. repeat msubst_simp.
-    split; [| split]. {
-      assert (Γ ⊢ tletapp v1 v2 e ⋮t (<[ A^a^v2 ] ρ [ B ]>)) by
-        eauto using term_type_check.
-      eapply tm_typing_regular_basic_typing in H.
-      eapply msubst_preserves_basic_typing_tm_empty in H; eauto.
-      repeat msubst_simp.
-      apply_eq H. cbn. eauto using pty_erase_msubst_eq.
-    } {
-      eapply_eq msubst_preserves_closed_hty_empty; eauto using wf_hty_closed.
-      repeat msubst_simp.
-    }
-    intros α β v HDα Hstepv.
-    apply reduction_tletapp in Hstepv.
-    destruct Hstepv as (βx & βe & v_x & -> & Hstepv_x & Hstepv).
-    auto_pose_fv x. repeat specialize_with x.
-    destruct HDv1 as (_ & _ & HDapp).
-    repeat rewrite_measure_irrelevant.
-    ospecialize* HDapp; eauto.
-    destruct HDapp as (_ & _ & HDapp). simpl in HDapp.
-    rewrite <- !msubst_open_am in HDapp by
-        (eauto using ctxRst_closed_env, ctxRst_lc).
-    rewrite <- !msubst_open_pty in HDapp by
-        (eauto using ctxRst_closed_env, ctxRst_lc).
-    ospecialize* HDapp; eauto.
-    destruct HDapp as [HDv_x HDα_βx].
-    assert (ctxRst (Γ ++ [(x, ρx ^p^ v2)]) (<[x:=v_x]> Γv)) as HΓv'. {
-      apply ctxRst_insert_easy; eauto. my_set_solver.
-    }
-    ospecialize* HDe; eauto.
-    rewrite <- msubst_intro_tm in HDe by
-        (eauto using ctxRst_closed_env, ctxRst_lc, ptyR_closed_value;
-         simpl_fv; my_set_solver).
-    repeat msubst_simp.
-    destruct HDe as (_ & _ & HDe).
-    rewrite msubst_insert_fresh_am in HDe;
-      eauto using ctxRst_closed_env, ptyR_closed_value.
-    2 : {
-      apply not_elem_of_union. split.
-      simpl_fv; my_set_solver.
-      eapply not_elem_of_weaken. 2: eauto using open_fv_am.
-      my_set_solver.
-    }
-    ospecialize* HDe; eauto.
-    repeat rewrite_measure_irrelevant.
-    rewrite msubst_insert_fresh_pty in HDe by
-      (eauto using ctxRst_closed_env, ptyR_closed_value;
-       simpl_fv; my_set_solver).
-    rewrite msubst_insert_fresh_am in HDe by
-      (eauto using ctxRst_closed_env, ptyR_closed_value;
-       simpl_fv; my_set_solver).
-    clear - HDe.
-    by simplify_list_eq.
-  (* [TEOpApp] *)
-  - intros Γ op v2 e ρ ρx ρ2 A A' B L HWF HTv2 HDv2 HTop HTe HDe Γv HΓv.
-    assert (∅ ⊢t (m{Γv}t) (tleteffop op v2 e) ⋮t ⌊ρ⌋) as HT. {
-      eapply msubst_preserves_basic_typing_tm_empty; eauto.
-      apply_eq tm_typing_regular_basic_typing; eauto using term_type_check.
-    }
-    assert (∅ ⊢t (m{Γv}t) (tletapp (value_of_op op) v2 e) ⋮t ⌊ρ⌋) as HTapp. {
-      repeat msubst_simp. rewrite msubst_value_of_op.
-      clear - HT.
-      sinvert HT. sinvert H5.
-      econstructor; eauto.
-      econstructor. instantiate_atom_listctx.
-      econstructor; eauto. econstructor. by simplify_map_eq.
-      instantiate_atom_listctx. simpl.
-      econstructor. econstructor. by simplify_map_eq.
-    }
-    eapply (htyR_refine _ (m{Γv}t (tletapp (value_of_op op) v2 e))). {
-      split; eauto.
-      repeat msubst_simp. rewrite msubst_value_of_op.
-      assert (body ((m{Γv}t) e)) as Hbody. {
-        sinvert HT. eexists. eauto using basic_typing_regular_tm.
-      }
-      clear - Hbody. intros * Hstepv.
-      apply reduction_tleteffop in Hstepv.
-      destruct Hstepv as (c2 & c_x & β' & -> & -> & Hred & Hstepv).
-      eapply_eq multistep_step. econstructor; eauto using lc.
-      unshelve (repeat econstructor); exact ∅.
-      econstructor. simpl. econstructor; eauto.
-      econstructor; eauto. by simplify_list_eq.
-      simpl. econstructor. econstructor; solve [eauto].
-      by simplify_list_eq. by simplify_list_eq.
-    }
-
-    eapply builtin_fundamental in HTop; eauto.
-    rewrite <- (msubst_value_of_op Γv) in HTop.
-    revert HTapp HTop. generalize (value_of_op op) as v1.
-    intros v1 HTapp HDv1.
-    ospecialize* HDv2; eauto. repeat msubst_simp.
-    split; [| split]. {
-      cbn. by rewrite <- pty_erase_msubst_eq.
-    } {
-      eapply_eq msubst_preserves_closed_hty_empty; eauto using wf_hty_closed.
-      repeat msubst_simp.
-    }
-    (* The rest of the proof is exactly the same as [TApp]. Maybe find a way to
-    abstract this and avoid copy-pasting. *)
-    intros α β v HDα Hstepv.
-    apply reduction_tletapp in Hstepv.
-    destruct Hstepv as (βx & βe & v_x & -> & Hstepv_x & Hstepv).
-    auto_pose_fv x. repeat specialize_with x.
-    destruct HDv1 as (_ & _ & HDapp).
-    repeat rewrite_measure_irrelevant.
-    ospecialize* HDapp; eauto.
-    destruct HDapp as (_ & _ & HDapp). simpl in HDapp.
-    rewrite <- !msubst_open_am in HDapp by
-        (eauto using ctxRst_closed_env, ctxRst_lc).
-    rewrite <- !msubst_open_pty in HDapp by
-        (eauto using ctxRst_closed_env, ctxRst_lc).
-    ospecialize* HDapp; eauto.
-    destruct HDapp as [HDv_x HDα_βx].
-    assert (ctxRst (Γ ++ [(x, ρx ^p^ v2)]) (<[x:=v_x]> Γv)) as HΓv'. {
-      apply ctxRst_insert_easy; eauto. my_set_solver.
-    }
-    ospecialize* HDe; eauto.
-    rewrite <- msubst_intro_tm in HDe by
-        (eauto using ctxRst_closed_env, ctxRst_lc, ptyR_closed_value;
-         simpl_fv; my_set_solver).
-    repeat msubst_simp.
-    destruct HDe as (_ & _ & HDe).
-    rewrite msubst_insert_fresh_am in HDe;
-      eauto using ctxRst_closed_env, ptyR_closed_value.
-    2 : {
-      apply not_elem_of_union. split.
-      simpl_fv; my_set_solver.
-      eapply not_elem_of_weaken. 2: eauto using open_fv_am.
-      my_set_solver.
-    }
-    ospecialize* HDe; eauto.
-    repeat rewrite_measure_irrelevant.
-    rewrite msubst_insert_fresh_pty in HDe by
-      (eauto using ctxRst_closed_env, ptyR_closed_value;
-       simpl_fv; my_set_solver).
-    rewrite msubst_insert_fresh_am in HDe by
-      (eauto using ctxRst_closed_env, ptyR_closed_value;
-       simpl_fv; my_set_solver).
-    clear - HDe.
-    by simplify_list_eq.
-  (* [TMatchb] *)
-  - intros Γ v e1 e2 ϕ τ L HWF HTv HDv HTe1 HDe1 HTe2 HDe2 Γv HΓv.
-    assert (∅ ⊢t (m{Γv}t) (tmatchb v e1 e2) ⋮t ⌊τ⌋) as HT by
-      qauto using term_type_check,
-                  tm_typing_regular_basic_typing,
-                  msubst_preserves_basic_typing_tm_empty.
-    auto_pose_fv x. repeat specialize_with x.
-    ospecialize* HDv; eauto.
-    repeat msubst_simp.
-    assert (exists (b : bool), m{Γv}v v = b) as [b He] by
-        qauto using value_typing_regular_basic_typing,
-                    msubst_preserves_basic_typing_value_empty,
-                    basic_typing_bool_canonical_form.
-    rewrite He in *.
-    assert (ctxRst
-              (Γ ++ [(x, {:TBool|(b0:c=b) & ((b0:v=v) & ϕ)})])
-              (<[x:=vconst b]>Γv)) as HΓv'. {
-      apply ctxRst_insert_easy; eauto. my_set_solver.
-      repeat msubst_simp.
-      repeat apply denote_base_pty_qualifier_and; eauto.
-      apply_eq mk_eq_constant_denote_pty. clear - HΓv.
-      rewrite_msubst msubst_qualifier. simpl. repeat msubst_simp.
-      apply_eq mk_eq_constant_denote_pty. clear - He HΓv.
-      rewrite_msubst msubst_qualifier. simpl. rewrite He. repeat msubst_simp.
-    }
-
-    destruct b.
-    + ospecialize* HDe1; eauto.
-      rewrite msubst_insert_fresh_tm in HDe1 by
-          (eauto using ctxRst_closed_env; simpl_fv; my_set_solver).
-      rewrite msubst_insert_fresh_hty in HDe1 by
-          (eauto using ctxRst_closed_env; simpl_fv; my_set_solver).
-      eapply htyR_refine; eauto.
-      split; eauto using reduction_matchb_true.
-      repeat esplit; eauto.
-      apply htyR_typed_closed in HDe1. destruct HDe1 as [HTe1' _].
-      rewrite <- hty_erase_msubst_eq in HTe1'. eauto.
-    + ospecialize* HDe2; eauto.
-      rewrite msubst_insert_fresh_tm in HDe2 by
-          (eauto using ctxRst_closed_env; simpl_fv; my_set_solver).
-      rewrite msubst_insert_fresh_hty in HDe2 by
-          (eauto using ctxRst_closed_env; simpl_fv; my_set_solver).
-      eapply htyR_refine; eauto.
-      split; eauto using reduction_matchb_false.
-      repeat esplit; eauto.
-      apply htyR_typed_closed in HDe2. destruct HDe2 as [HTe2' _].
-      rewrite <- hty_erase_msubst_eq in HTe2'. eauto.
-Qed.
-
-(** Fundamental theorem for value typing *)
-Theorem fundamental_value:
-  well_formed_builtin_typing ->
-  forall (Γ: listctx pty) (v: value) (ρ: pty),
-    Γ ⊢ v ⋮v ρ ->
-    forall Γv, ctxRst Γ Γv -> p⟦ m{Γv}p ρ ⟧ (m{Γv}v v).
-Proof.
-  qauto using fundamental_combined.
-Qed.
-
-(** Fundamental theorem (Theorem 4.8) *)
-Theorem fundamental:
-  well_formed_builtin_typing ->
-  forall (Γ: listctx pty) (e: tm) (τ: hty),
-    Γ ⊢ e ⋮t τ ->
-    forall σ, ctxRst Γ σ -> ⟦ m{ σ }h τ ⟧ (m{ σ }t e).
-Proof.
-  qauto using fundamental_combined.
-Qed.
-
-Transparent msubst.
-
-(** A general type soundness theorem *)
-Corollary soundness' :
-  well_formed_builtin_typing ->
-  forall (e : tm) (ρ : pty) (A : am),
-    [] ⊢ e ⋮t (<[ A ] ρ [ A ]>) ->
-    forall (v : value) α α',
-      a⟦ A ⟧ α ->
-      α ⊧ e ↪*{ α' } v ->
-      p⟦ ρ ⟧ v /\ a⟦ A ⟧ (α ++ α').
-Proof.
-  intros HWF * HT * HDα Hstepv.
-  eapply fundamental in HT; eauto using ctxRst.
-  unfold msubst in HT. rewrite !map_fold_empty in HT.
-  qauto using HT.
-Qed.
-
-(** Type soundness (Corollary 4.9) *)
-Corollary soundness :
-  well_formed_builtin_typing ->
-  forall (f: value) (b_x b_y: base_ty) (t: pty) (A: am),
-    [] ⊢ f ⋮v (b_x⇢(mk_top b_y)⇨(<[ A ] t [ A ]>)) ->
-    forall v_x v_y,
-      ∅ ⊢t v_x ⋮v b_x ->
-      ∅ ⊢t v_y ⋮v b_y ->
-      forall (v : value) α α',
-        a⟦ {0 ~a> v_y} ({1 ~a> v_x} A) ⟧ α ->
-        α ⊧ (mk_app_e_v f v_y) ↪*{ α' } v ->
-        a⟦ {0 ~a> v_y} ({1 ~a> v_x} A) ⟧ (α ++ α') /\
-          p⟦ {0 ~p> v_y} ({1 ~p> v_x} t) ⟧ v.
-Proof.
-  intros HWF * HT * HTv_x HTv_y * HDα Hstepv.
-  eapply fundamental_value in HT; eauto using ctxRst.
-  unfold msubst in HT. rewrite !map_fold_empty in HT.
-  destruct HT as (_&_&HD); eauto.
-  repeat rewrite_measure_irrelevant.
-  specialize (HD _ HTv_x).
-  simpl pty_open in HD.
-  destruct HD as (_&_&HD).
-  repeat rewrite_measure_irrelevant.
-  apply and_comm.
-  eapply HD; eauto using mk_top_denote_pty.
-Qed.
-
-Print Assumptions soundness.
