Fundamental.v
@@ -1,0 +1,504 @@
+From stdpp Require Import mapset.
+From CT Require Import CoreLangProp.
+From CT Require Import OperationalSemantics.
+From CT Require Import BasicTypingProp.
+From CT Require Import TransducerProp.
+From CT Require Import RefinementTypeProp.
+From CT Require Import Denotation.
+From CT Require Import InstantiationProp.
+From CT Require Import Typing.
+
+Import Atom.
+Import CoreLang.
+Import Tactics.
+Import NamelessTactics.
+Import ListCtx.
+Import Trace.
+Import OperationalSemantics.
+Import BasicTyping.
+Import Qualifier.
+Import Transducer.
+Import RefinementType.
+Import Denotation.
+Import Instantiation.
+Import Typing.
+
+(** * Main metatheoretic results *)
+
+(** Convert an event operator to a value:
+  [op] is [fun x => leteffop y = op x in y] *)
+Definition value_of_op op : value :=
+  vlam TNat (tleteffop op (vbvar 0) (vbvar 0)).
+
+(** Well-formed built-in operator typing context (Definition 4.7) *)
+(* We simply treat the event operator as a value. This is equivalent to the
+definition in the paper (if we expand the denotation of this value). *)
+Definition well_formed_builtin_typing :=
+  forall op ρ,
+    builtin_typing_relation op ρ ->
+    ⟦ ρ ⟧ (value_of_op op).
+
+Lemma msubst_value_of_op Γv op :
+  m{Γv}v (value_of_op op) = value_of_op op.
+Proof.
+  rewrite msubst_fresh_value. eauto.
+  my_set_solver.
+Qed.
+
+Lemma value_of_op_regular_basic_typing op:
+  ∅ ⊢t value_of_op op ⋮v ty_of_op op.
+Proof.
+  econstructor.
+  simpl. instantiate (1:=∅). intros.
+  econstructor. econstructor. simplify_map_eq. reflexivity. reflexivity.
+  instantiate_atom_listctx.
+  simpl. econstructor. econstructor. simplify_map_eq. reflexivity.
+Qed.
+
+(* At some point the proof is very slow without marking [msubst] opaque. *)
+Opaque msubst.
+
+Ltac simpl_fv :=
+  do_hyps (fun H => try match type of H with
+                    | _ ∉ _ =>
+                        simpl in H; rewrite ?ctxRst_dom in H by eassumption
+                    end).
+
+(** Fundamental theorem for event operator typing *)
+Lemma builtin_fundamental:
+  well_formed_builtin_typing ->
+  forall (Γ: listctx rty) (op: effop) (ρ : rty),
+    Γ ⊢ op ⋮o ρ ->
+    forall Γv, ctxRst Γ Γv -> ⟦ m{ Γv }r ρ ⟧ (value_of_op op).
+Proof.
+  intros HWF Γ op ρ Hop Γv HΓv. sinvert Hop.
+  apply H1; eauto.
+  apply HWF in H0.
+  rewrite msubst_fresh_rty; eauto.
+  apply rtyR_typed_closed in H0. simp_hyps.
+  sinvert H3.
+  my_set_solver.
+Qed.
+
+Check closed_rty_fine.
+
+Ltac fine_solver :=
+  repeat (match goal with
+          | [ H: _ ⊢WF _ |- pure_rty _ ] =>
+              apply closed_rty_fine in H; eauto; simpl in H; intuition; eauto
+          | [ H: _ ⊢WF _ |- fine_rty _ ] =>
+              apply closed_rty_fine in H; eauto; simpl in H;intuition; eauto
+          end).
+  (* match goal with *)
+  (* | [ H: _ |- fine_rty _ ] => simpl in *; eauto *)
+  (* end. *)
+
+(** Combined fundamental theorem for value typing (refinemnet types) and term
+  typing (Hoare automata types) *)
+Theorem fundamental_combined:
+  well_formed_builtin_typing ->
+  (forall (Γ: listctx rty) (v: value) (ρ: rty),
+    Γ ⊢ v ⋮v ρ ->
+    forall Γv, ctxRst Γ Γv -> ⟦ m{Γv}r ρ ⟧ (m{Γv}v v)) /\
+  (forall (Γ: listctx rty) (e: tm) (τ: rty),
+    Γ ⊢ e ⋮t τ ->
+    forall Γv, ctxRst Γ Γv -> ⟦ m{ Γv }r τ ⟧ (m{ Γv }t e)).
+Proof.
+  intros HWFbuiltin.
+  apply value_term_type_check_mutind.
+  (* [TSubPP] *)
+  - intros Γ v ρ1 ρ2 HWFρ2 _ HDρ1 Hsub Γv HΓv. specialize (HDρ1 _ HΓv).
+    apply Hsub in HDρ1; auto.
+  (* [TConst] *)
+  - intros Γ c HWF Γv HΓv. repeat msubst_simp. eauto using mk_eq_constant_denote_rty.
+  (* [TBaseVar] *)
+  - intros Γ x b ϕ Hwf Hfind Γv HΓv.
+    dup_hyp HΓv (fun H => eapply ctxRst_ctxfind in H; eauto). simp_hyps.
+    repeat msubst_simp. rewrite H0.
+    destruct H1 as [H _].
+    sinvert H. cbn in H3.
+    dup_hyp H3 (fun H => apply basic_typing_base_canonical_form in H).
+    simp_hyps. subst. sinvert H3.
+    eauto using mk_eq_constant_denote_rty. fine_solver.
+  (* [TFuncVar] *)
+  - intros Γ x ρ τ Hwf Hfind Γv HΓv.
+    dup_hyp HΓv (fun H => eapply ctxRst_ctxfind in H; eauto). simp_hyps.
+    repeat msubst_simp.
+    by rewrite H0. fine_solver.
+  (* [TFun] *)
+  - intros Γ Tx ρ e τ L HWF Ht HDe He Γv HΓv. repeat msubst_simp.
+    eapply denotation_application_lam; eauto.
+    cbn. repeat rewrite <- rty_erase_msubst_eq. subst. eauto.
+    {
+      assert (Γ ⊢ vlam Tx e ⋮v (ρ⇨τ)) by eauto using value_type_check.
+      eapply value_typing_regular_basic_typing in H.
+      eapply msubst_preserves_basic_typing_value_empty in H; eauto.
+      repeat msubst_simp.
+      econstructor. apply_eq H. cbn. subst. reflexivity.
+    } {
+      eapply_eq msubst_preserves_closed_rty_empty; eauto.
+      msubst_simp.
+    }
+    intros v_x Hv_x.
+    auto_pose_fv x. repeat specialize_with x.
+    assert (ctxRst (Γ ++ [(x, ρ)]) (<[x:=v_x]> Γv)) as HΓv'. {
+      apply ctxRst_insert_easy; eauto. my_set_solver. fine_solver.
+    }
+    ospecialize* HDe; eauto.
+    rewrite <- msubst_intro_tm in HDe by
+        (eauto using ctxRst_closed_env, ctxRst_lc, rtyR_closed_value;
+         simpl_fv; my_set_solver).
+    rewrite <- msubst_intro_rty in HDe by
+        (eauto using ctxRst_closed_env, ctxRst_lc, rtyR_closed_value;
+         simpl_fv; my_set_solver).
+    eauto.
+  (* [TFix] *)
+  - intros Γ Tx ϕ e τ T L HWF Hlam HDlam He Γv HΓv. repeat msubst_simp.
+    eapply denotation_application_fixed; eauto.
+    by rewrite <- rty_erase_msubst_eq.
+    {
+      assert (Γ ⊢ vfix (Tx ⤍ T) (vlam (Tx ⤍ T) e) ⋮v ({:Tx|ϕ}⇨τ))
+        by eauto using value_type_check.
+      eapply value_typing_regular_basic_typing in H.
+      eapply msubst_preserves_basic_typing_value_empty in H; eauto.
+      repeat msubst_simp.
+      apply_eq H. cbn. subst. eauto.
+    } {
+      eapply_eq msubst_preserves_closed_rty_empty; eauto.
+      repeat msubst_simp.
+    }
+    intros v_x Hv_x.
+    auto_pose_fv x. repeat specialize_with x.
+    assert (ctxRst (Γ ++ [(x, {:Tx|ϕ})]) (<[x:=v_x]> Γv)) as HΓv'. {
+      apply ctxRst_insert_easy; eauto. my_set_solver.
+      msubst_simp. fine_solver.
+    }
+    ospecialize* HDlam; eauto.
+    rewrite <- msubst_intro_value in HDlam by
+        (eauto using ctxRst_closed_env, ctxRst_lc, rtyR_closed_value;
+         simpl_fv; my_set_solver).
+    repeat msubst_simp.
+    rewrite <- msubst_intro_rty in HDlam by
+        (eauto using ctxRst_closed_env, ctxRst_lc, rtyR_closed_value;
+         simpl_fv; my_set_solver).
+    rewrite msubst_insert_fresh_rty in HDlam by
+      (eauto using ctxRst_closed_env, rtyR_closed_value; simpl_fv; my_set_solver).
+    rewrite_msubst msubst_qualifier in HDlam.
+    rewrite msubst_insert_fresh_qualifier in HDlam by
+      (eauto using ctxRst_closed_env, rtyR_closed_value; simpl_fv; my_set_solver).
+    apply_eq HDlam.
+    simpl. repeat msubst_simp.
+    clear. simplify_map_eq. eauto.
+  (* [TEPur] *)
+  - intros Γ v ρ HWF Hv HDv Γv HΓv. specialize (HDv _ HΓv).
+    repeat msubst_simp.
+    split; [| split]. {
+      eapply value_typing_regular_basic_typing in Hv.
+      eapply msubst_preserves_basic_typing_value_empty in Hv; eauto.
+      cbn. rewrite <- rty_erase_msubst_eq. eauto.
+    } {
+      eapply_eq msubst_preserves_closed_rty_empty; eauto.
+      repeat msubst_simp.
+    }
+    admit.
+  (* [TSub] *)
+  - intros Γ e τ1 τ2 HWFτ2 _ HDτ1 Hsub Γv HΓv. specialize (HDτ1 _ HΓv).
+    apply Hsub in HDτ1; auto.
+  (* [TLetE] *)
+  - intros Γ e_x e ρx ρ A A' B L HWF HTe_x HDe_x HTe HDe Γv HΓv.
+    ospecialize* HDe_x; eauto. repeat msubst_simp.
+    split; [| split]. {
+      assert (Γ ⊢ tlete e_x e ⋮t (<[ A ] ρ [ B ]>)) by eauto using term_type_check.
+      eapply tm_typing_regular_basic_typing in H.
+      eapply msubst_preserves_basic_typing_tm_empty in H; eauto.
+      repeat msubst_simp.
+      apply_eq H. cbn. eauto using rty_erase_msubst_eq.
+    } {
+      eapply_eq msubst_preserves_closed_rty_empty; eauto using wf_rty_closed.
+      repeat msubst_simp.
+    }
+    intros α β v HDα Hstepv.
+    apply reduction_tlete in Hstepv.
+    destruct Hstepv as (βx & βe & v_x & -> & Hstepv_x & Hstepv).
+    auto_pose_fv x. repeat specialize_with x.
+    destruct HDe_x as (_ & _ & HDe_x).
+    ospecialize* HDe_x; eauto. destruct HDe_x as [HDv_x HDα_βx].
+    assert (ctxRst (Γ ++ [(x, ρx)]) (<[x:=v_x]> Γv)) as HΓv'. {
+      apply ctxRst_insert_easy; eauto. my_set_solver.
+    }
+    ospecialize* HDe; eauto.
+    rewrite <- msubst_intro_tm in HDe by
+        (eauto using ctxRst_closed_env, ctxRst_lc, rtyR_closed_value;
+         simpl_fv; my_set_solver).
+    repeat msubst_simp.
+    destruct HDe as (_ & _ & HDe).
+    rewrite msubst_insert_fresh_am in HDe by
+      (eauto using ctxRst_closed_env, rtyR_closed_value;
+       simpl_fv; my_set_solver).
+    ospecialize* HDe; eauto.
+    repeat rewrite_measure_irrelevant.
+    rewrite msubst_insert_fresh_rty in HDe by
+      (eauto using ctxRst_closed_env, rtyR_closed_value;
+       simpl_fv; my_set_solver).
+    rewrite msubst_insert_fresh_am in HDe by
+      (eauto using ctxRst_closed_env, rtyR_closed_value;
+       simpl_fv; my_set_solver).
+    clear - HDe.
+    by simplify_list_eq.
+  (* [TApp] *)
+  - intros Γ v1 v2 e ρ ρx ρ2 A A' B L HWF HTv2 HDv2 HTv1 HDv1 HTe HDe Γv HΓv.
+    ospecialize* HDv1; eauto. ospecialize* HDv2; eauto. repeat msubst_simp.
+    split; [| split]. {
+      assert (Γ ⊢ tletapp v1 v2 e ⋮t (<[ A^a^v2 ] ρ [ B ]>)) by
+        eauto using term_type_check.
+      eapply tm_typing_regular_basic_typing in H.
+      eapply msubst_preserves_basic_typing_tm_empty in H; eauto.
+      repeat msubst_simp.
+      apply_eq H. cbn. eauto using rty_erase_msubst_eq.
+    } {
+      eapply_eq msubst_preserves_closed_rty_empty; eauto using wf_rty_closed.
+      repeat msubst_simp.
+    }
+    intros α β v HDα Hstepv.
+    apply reduction_tletapp in Hstepv.
+    destruct Hstepv as (βx & βe & v_x & -> & Hstepv_x & Hstepv).
+    auto_pose_fv x. repeat specialize_with x.
+    destruct HDv1 as (_ & _ & HDapp).
+    repeat rewrite_measure_irrelevant.
+    ospecialize* HDapp; eauto.
+    destruct HDapp as (_ & _ & HDapp). simpl in HDapp.
+    rewrite <- !msubst_open_am in HDapp by
+        (eauto using ctxRst_closed_env, ctxRst_lc).
+    rewrite <- !msubst_open_rty in HDapp by
+        (eauto using ctxRst_closed_env, ctxRst_lc).
+    ospecialize* HDapp; eauto.
+    destruct HDapp as [HDv_x HDα_βx].
+    assert (ctxRst (Γ ++ [(x, ρx ^p^ v2)]) (<[x:=v_x]> Γv)) as HΓv'. {
+      apply ctxRst_insert_easy; eauto. my_set_solver.
+    }
+    ospecialize* HDe; eauto.
+    rewrite <- msubst_intro_tm in HDe by
+        (eauto using ctxRst_closed_env, ctxRst_lc, rtyR_closed_value;
+         simpl_fv; my_set_solver).
+    repeat msubst_simp.
+    destruct HDe as (_ & _ & HDe).
+    rewrite msubst_insert_fresh_am in HDe;
+      eauto using ctxRst_closed_env, rtyR_closed_value.
+    2 : {
+      apply not_elem_of_union. split.
+      simpl_fv; my_set_solver.
+      eapply not_elem_of_weaken. 2: eauto using open_fv_am.
+      my_set_solver.
+    }
+    ospecialize* HDe; eauto.
+    repeat rewrite_measure_irrelevant.
+    rewrite msubst_insert_fresh_rty in HDe by
+      (eauto using ctxRst_closed_env, rtyR_closed_value;
+       simpl_fv; my_set_solver).
+    rewrite msubst_insert_fresh_am in HDe by
+      (eauto using ctxRst_closed_env, rtyR_closed_value;
+       simpl_fv; my_set_solver).
+    clear - HDe.
+    by simplify_list_eq.
+  (* [TEOpApp] *)
+  - intros Γ op v2 e ρ ρx ρ2 A A' B L HWF HTv2 HDv2 HTop HTe HDe Γv HΓv.
+    assert (∅ ⊢t (m{Γv}t) (tleteffop op v2 e) ⋮t ⌊ρ⌋) as HT. {
+      eapply msubst_preserves_basic_typing_tm_empty; eauto.
+      apply_eq tm_typing_regular_basic_typing; eauto using term_type_check.
+    }
+    assert (∅ ⊢t (m{Γv}t) (tletapp (value_of_op op) v2 e) ⋮t ⌊ρ⌋) as HTapp. {
+      repeat msubst_simp. rewrite msubst_value_of_op.
+      clear - HT.
+      sinvert HT. sinvert H5.
+      econstructor; eauto.
+      econstructor. instantiate_atom_listctx.
+      econstructor; eauto. econstructor. by simplify_map_eq.
+      instantiate_atom_listctx. simpl.
+      econstructor. econstructor. by simplify_map_eq.
+    }
+    eapply (rtyR_refine _ (m{Γv}t (tletapp (value_of_op op) v2 e))). {
+      split; eauto.
+      repeat msubst_simp. rewrite msubst_value_of_op.
+      assert (body ((m{Γv}t) e)) as Hbody. {
+        sinvert HT. eexists. eauto using basic_typing_regular_tm.
+      }
+      clear - Hbody. intros * Hstepv.
+      apply reduction_tleteffop in Hstepv.
+      destruct Hstepv as (c2 & c_x & β' & -> & -> & Hred & Hstepv).
+      eapply_eq multistep_step. econstructor; eauto using lc.
+      unshelve (repeat econstructor); exact ∅.
+      econstructor. simpl. econstructor; eauto.
+      econstructor; eauto. by simplify_list_eq.
+      simpl. econstructor. econstructor; solve [eauto].
+      by simplify_list_eq. by simplify_list_eq.
+    }
+
+    eapply builtin_fundamental in HTop; eauto.
+    rewrite <- (msubst_value_of_op Γv) in HTop.
+    revert HTapp HTop. generalize (value_of_op op) as v1.
+    intros v1 HTapp HDv1.
+    ospecialize* HDv2; eauto. repeat msubst_simp.
+    split; [| split]. {
+      cbn. by rewrite <- rty_erase_msubst_eq.
+    } {
+      eapply_eq msubst_preserves_closed_rty_empty; eauto using wf_rty_closed.
+      repeat msubst_simp.
+    }
+    (* The rest of the proof is exactly the same as [TApp]. Maybe find a way to
+    abstract this and avoid copy-pasting. *)
+    intros α β v HDα Hstepv.
+    apply reduction_tletapp in Hstepv.
+    destruct Hstepv as (βx & βe & v_x & -> & Hstepv_x & Hstepv).
+    auto_pose_fv x. repeat specialize_with x.
+    destruct HDv1 as (_ & _ & HDapp).
+    repeat rewrite_measure_irrelevant.
+    ospecialize* HDapp; eauto.
+    destruct HDapp as (_ & _ & HDapp). simpl in HDapp.
+    rewrite <- !msubst_open_am in HDapp by
+        (eauto using ctxRst_closed_env, ctxRst_lc).
+    rewrite <- !msubst_open_rty in HDapp by
+        (eauto using ctxRst_closed_env, ctxRst_lc).
+    ospecialize* HDapp; eauto.
+    destruct HDapp as [HDv_x HDα_βx].
+    assert (ctxRst (Γ ++ [(x, ρx ^p^ v2)]) (<[x:=v_x]> Γv)) as HΓv'. {
+      apply ctxRst_insert_easy; eauto. my_set_solver.
+    }
+    ospecialize* HDe; eauto.
+    rewrite <- msubst_intro_tm in HDe by
+        (eauto using ctxRst_closed_env, ctxRst_lc, rtyR_closed_value;
+         simpl_fv; my_set_solver).
+    repeat msubst_simp.
+    destruct HDe as (_ & _ & HDe).
+    rewrite msubst_insert_fresh_am in HDe;
+      eauto using ctxRst_closed_env, rtyR_closed_value.
+    2 : {
+      apply not_elem_of_union. split.
+      simpl_fv; my_set_solver.
+      eapply not_elem_of_weaken. 2: eauto using open_fv_am.
+      my_set_solver.
+    }
+    ospecialize* HDe; eauto.
+    repeat rewrite_measure_irrelevant.
+    rewrite msubst_insert_fresh_rty in HDe by
+      (eauto using ctxRst_closed_env, rtyR_closed_value;
+       simpl_fv; my_set_solver).
+    rewrite msubst_insert_fresh_am in HDe by
+      (eauto using ctxRst_closed_env, rtyR_closed_value;
+       simpl_fv; my_set_solver).
+    clear - HDe.
+    by simplify_list_eq.
+  (* [TMatchb] *)
+  - intros Γ v e1 e2 ϕ τ L HWF HTv HDv HTe1 HDe1 HTe2 HDe2 Γv HΓv.
+    assert (∅ ⊢t (m{Γv}t) (tmatchb v e1 e2) ⋮t ⌊τ⌋) as HT by
+      qauto using term_type_check,
+                  tm_typing_regular_basic_typing,
+                  msubst_preserves_basic_typing_tm_empty.
+    auto_pose_fv x. repeat specialize_with x.
+    ospecialize* HDv; eauto.
+    repeat msubst_simp.
+    assert (exists (b : bool), m{Γv}v v = b) as [b He] by
+        qauto using value_typing_regular_basic_typing,
+                    msubst_preserves_basic_typing_value_empty,
+                    basic_typing_bool_canonical_form.
+    rewrite He in *.
+    assert (ctxRst
+              (Γ ++ [(x, {:TBool|(b0:c=b) & ((b0:v=v) & ϕ)})])
+              (<[x:=vconst b]>Γv)) as HΓv'. {
+      apply ctxRst_insert_easy; eauto. my_set_solver.
+      repeat msubst_simp.
+      repeat apply denote_base_rty_qualifier_and; eauto.
+      apply_eq mk_eq_constant_denote_rty. clear - HΓv.
+      rewrite_msubst msubst_qualifier. simpl. repeat msubst_simp.
+      apply_eq mk_eq_constant_denote_rty. clear - He HΓv.
+      rewrite_msubst msubst_qualifier. simpl. rewrite He. repeat msubst_simp.
+    }
+
+    destruct b.
+    + ospecialize* HDe1; eauto.
+      rewrite msubst_insert_fresh_tm in HDe1 by
+          (eauto using ctxRst_closed_env; simpl_fv; my_set_solver).
+      rewrite msubst_insert_fresh_rty in HDe1 by
+          (eauto using ctxRst_closed_env; simpl_fv; my_set_solver).
+      eapply rtyR_refine; eauto.
+      split; eauto using reduction_matchb_true.
+      repeat esplit; eauto.
+      apply rtyR_typed_closed in HDe1. destruct HDe1 as [HTe1' _].
+      rewrite <- rty_erase_msubst_eq in HTe1'. eauto.
+    + ospecialize* HDe2; eauto.
+      rewrite msubst_insert_fresh_tm in HDe2 by
+          (eauto using ctxRst_closed_env; simpl_fv; my_set_solver).
+      rewrite msubst_insert_fresh_rty in HDe2 by
+          (eauto using ctxRst_closed_env; simpl_fv; my_set_solver).
+      eapply rtyR_refine; eauto.
+      split; eauto using reduction_matchb_false.
+      repeat esplit; eauto.
+      apply rtyR_typed_closed in HDe2. destruct HDe2 as [HTe2' _].
+      rewrite <- rty_erase_msubst_eq in HTe2'. eauto.
+Qed.
+
+(** Fundamental theorem for value typing *)
+Theorem fundamental_value:
+  well_formed_builtin_typing ->
+  forall (Γ: listctx rty) (v: value) (ρ: rty),
+    Γ ⊢ v ⋮v ρ ->
+    forall Γv, ctxRst Γ Γv -> p⟦ m{Γv}p ρ ⟧ (m{Γv}v v).
+Proof.
+  qauto using fundamental_combined.
+Qed.
+
+(** Fundamental theorem (Theorem 4.8) *)
+Theorem fundamental:
+  well_formed_builtin_typing ->
+  forall (Γ: listctx rty) (e: tm) (τ: rty),
+    Γ ⊢ e ⋮t τ ->
+    forall σ, ctxRst Γ σ -> ⟦ m{ σ }h τ ⟧ (m{ σ }t e).
+Proof.
+  qauto using fundamental_combined.
+Qed.
+
+Transparent msubst.
+
+(** A general type soundness theorem *)
+Corollary soundness' :
+  well_formed_builtin_typing ->
+  forall (e : tm) (ρ : rty) (A : am),
+    [] ⊢ e ⋮t (<[ A ] ρ [ A ]>) ->
+    forall (v : value) α α',
+      a⟦ A ⟧ α ->
+      α ⊧ e ↪*{ α' } v ->
+      p⟦ ρ ⟧ v /\ a⟦ A ⟧ (α ++ α').
+Proof.
+  intros HWF * HT * HDα Hstepv.
+  eapply fundamental in HT; eauto using ctxRst.
+  unfold msubst in HT. rewrite !map_fold_empty in HT.
+  qauto using HT.
+Qed.
+
+(** Type soundness (Corollary 4.9) *)
+Corollary soundness :
+  well_formed_builtin_typing ->
+  forall (f: value) (b_x b_y: base_ty) (t: rty) (A: am),
+    [] ⊢ f ⋮v (b_x⇢(mk_top b_y)⇨(<[ A ] t [ A ]>)) ->
+    forall v_x v_y,
+      ∅ ⊢t v_x ⋮v b_x ->
+      ∅ ⊢t v_y ⋮v b_y ->
+      forall (v : value) α α',
+        a⟦ {0 ~a> v_y} ({1 ~a> v_x} A) ⟧ α ->
+        α ⊧ (mk_app_e_v f v_y) ↪*{ α' } v ->
+        a⟦ {0 ~a> v_y} ({1 ~a> v_x} A) ⟧ (α ++ α') /\
+          p⟦ {0 ~p> v_y} ({1 ~p> v_x} t) ⟧ v.
+Proof.
+  intros HWF * HT * HTv_x HTv_y * HDα Hstepv.
+  eapply fundamental_value in HT; eauto using ctxRst.
+  unfold msubst in HT. rewrite !map_fold_empty in HT.
+  destruct HT as (_&_&HD); eauto.
+  repeat rewrite_measure_irrelevant.
+  specialize (HD _ HTv_x).
+  simpl rty_open in HD.
+  destruct HD as (_&_&HD).
+  repeat rewrite_measure_irrelevant.
+  apply and_comm.
+  eapply HD; eauto using mk_top_denote_rty.
+Qed.
+
+Print Assumptions soundness.
